<?xml version="1.0"?>
<rdf:RDF xmlns="http://purl.obolibrary.org/obo/DASH-Onto.owl#"
     xml:base="http://purl.obolibrary.org/obo/DASH-Onto.owl"
     xmlns:obo="http://purl.obolibrary.org/obo/"
     xmlns:owl="http://www.w3.org/2002/07/owl#"
     xmlns:rdf="http://www.w3.org/1999/02/22-rdf-syntax-ns#"
     xmlns:xml="http://www.w3.org/XML/1998/namespace"
     xmlns:xsd="http://www.w3.org/2001/XMLSchema#"
     xmlns:rdfs="http://www.w3.org/2000/01/rdf-schema#"
     xmlns:terms="http://purl.org/dc/terms/">
    <owl:Ontology rdf:about="http://purl.obolibrary.org/obo/DASH-Onto.owl">
        <terms:description xml:lang="en">None</terms:description>
        <terms:license rdf:resource="https://creativecommons.org/licenses/unspecified"/>
        <terms:title xml:lang="en">Data Access Support Hub Ontology</terms:title>
        <owl:versionInfo>2024-01-16</owl:versionInfo>
    </owl:Ontology>
    


    <!-- 
    ///////////////////////////////////////////////////////////////////////////////////////
    //
    // Annotation properties
    //
    ///////////////////////////////////////////////////////////////////////////////////////
     -->

    


    <!-- http://purl.obolibrary.org/obo/IAO_0000115 -->

    <owl:AnnotationProperty rdf:about="http://purl.obolibrary.org/obo/IAO_0000115">
        <rdfs:isDefinedBy rdf:resource="http://purl.obolibrary.org/obo/iao.owl"/>
        <rdfs:label xml:lang="en">definition</rdfs:label>
    </owl:AnnotationProperty>
    


    <!-- http://purl.org/dc/terms/description -->

    <owl:AnnotationProperty rdf:about="http://purl.org/dc/terms/description"/>
    


    <!-- http://purl.org/dc/terms/license -->

    <owl:AnnotationProperty rdf:about="http://purl.org/dc/terms/license"/>
    


    <!-- http://purl.org/dc/terms/title -->

    <owl:AnnotationProperty rdf:about="http://purl.org/dc/terms/title"/>
    


    <!-- 
    ///////////////////////////////////////////////////////////////////////////////////////
    //
    // Classes
    //
    ///////////////////////////////////////////////////////////////////////////////////////
     -->

    


    <!-- http://purl.obolibrary.org/obo/DASH-Onto_0000004 -->

    <owl:Class rdf:about="http://purl.obolibrary.org/obo/DASH-Onto_0000004">
        <obo:IAO_0000115 xml:lang="en">An agreement drafting that is TBD.</obo:IAO_0000115>
        <rdfs:comment xml:lang="en">Ont/glossary: proposed.</rdfs:comment>
        <rdfs:label xml:lang="en">DC Agreement drafting</rdfs:label>
    </owl:Class>
    


    <!-- http://purl.obolibrary.org/obo/DASH-Onto_0000005 -->

    <owl:Class rdf:about="http://purl.obolibrary.org/obo/DASH-Onto_0000005">
        <obo:IAO_0000115 xml:lang="en">An agreement drafting that is TBD.</obo:IAO_0000115>
        <rdfs:comment xml:lang="en">Ont/glossary: proposed.</rdfs:comment>
        <rdfs:label xml:lang="en">TEA Agreement drafting</rdfs:label>
    </owl:Class>
    


    <!-- http://purl.obolibrary.org/obo/DASH-Onto_0000007 -->

    <owl:Class rdf:about="http://purl.obolibrary.org/obo/DASH-Onto_0000007">
        <obo:IAO_0000115 xml:lang="en">An agreement signature where the required parties are a data custodian and a project research group.</obo:IAO_0000115>
        <rdfs:comment xml:lang="en">Ont: proposed to cover DC/TEA bifurcation.</rdfs:comment>
        <rdfs:label xml:lang="en">DC Agreement signature</rdfs:label>
    </owl:Class>
    


    <!-- http://purl.obolibrary.org/obo/DASH-Onto_0000008 -->

    <owl:Class rdf:about="http://purl.obolibrary.org/obo/DASH-Onto_0000008">
        <obo:IAO_0000115 xml:lang="en">An agreement signature where the required parties are those data custodians contributing to the TEA and a project research group.</obo:IAO_0000115>
        <rdfs:comment xml:lang="en">Ont: proposed to cover DC/TEA bifurcation.</rdfs:comment>
        <rdfs:label xml:lang="en">TEA Agreement signature</rdfs:label>
    </owl:Class>
    


    <!-- http://purl.obolibrary.org/obo/DASH-Onto_0000013 -->

    <owl:Class rdf:about="http://purl.obolibrary.org/obo/DASH-Onto_0000013">
        <obo:IAO_0000115 xml:lang="en">A process by which a DASH User acquires information about metadata, data metrics and data provenance elements of data items, as well as selection functions.</obo:IAO_0000115>
        <rdfs:comment xml:lang="en">DASH: DASH Guidance: Data Exploration (DATX)</rdfs:comment>
        <rdfs:comment xml:lang="en">Glossary: &apos;guided data exploration&apos;</rdfs:comment>
        <rdfs:label xml:lang="en">DASH Data advice</rdfs:label>
    </owl:Class>
    


    <!-- http://purl.obolibrary.org/obo/DASH-Onto_0000014 -->

    <owl:Class rdf:about="http://purl.obolibrary.org/obo/DASH-Onto_0000014">
        <obo:IAO_0000115 xml:lang="en">A process by which a DASH User acquires information about services offered by a data custodian.</obo:IAO_0000115>
        <rdfs:comment xml:lang="en">DASH: DASH Guidance: Support Exploration (SUPX)</rdfs:comment>
        <rdfs:comment xml:lang="en">Glossary: &apos;guided support exploration&apos;</rdfs:comment>
        <rdfs:label xml:lang="en">DASH Support advice</rdfs:label>
    </owl:Class>
    


    <!-- http://purl.obolibrary.org/obo/DASH-Onto_0000015 -->

    <owl:Class rdf:about="http://purl.obolibrary.org/obo/DASH-Onto_0000015">
        <obo:IAO_0000115 xml:lang="en">A DASH project advice that is TBD.</obo:IAO_0000115>
        <rdfs:comment xml:lang="en">Ont: proposed.</rdfs:comment>
        <rdfs:label xml:lang="en">Scored data custodian cost</rdfs:label>
    </owl:Class>
    


    <!-- http://purl.obolibrary.org/obo/DASH-Onto_0000016 -->

    <owl:Class rdf:about="http://purl.obolibrary.org/obo/DASH-Onto_0000016">
        <obo:IAO_0000115 xml:lang="en">A process by which a DASH User acquires information about eligibility requirements from a data custodian.</obo:IAO_0000115>
        <rdfs:comment xml:lang="en">DASH: DASH Guidance: DASH Eligibility (DEL)</rdfs:comment>
        <rdfs:comment xml:lang="en">Glossary: &apos;guided eligibility exploration&apos;</rdfs:comment>
        <rdfs:label xml:lang="en">DASH eligibility advice</rdfs:label>
    </owl:Class>
    


    <!-- http://purl.obolibrary.org/obo/DASH-Onto_0000019 -->

    <owl:Class rdf:about="http://purl.obolibrary.org/obo/DASH-Onto_0000019">
        <obo:IAO_0000115 xml:lang="en">A DASH activity that is TBD.</obo:IAO_0000115>
        <rdfs:comment xml:lang="en">DASH: DASH Q&amp;A (QUEST)</rdfs:comment>
        <rdfs:comment xml:lang="en">DASH: Guidance catch-all (DG)</rdfs:comment>
        <rdfs:comment xml:lang="en">DASH: Project on hold (PHOLD)</rdfs:comment>
        <rdfs:comment xml:lang="en">DASH: issues (ISS)</rdfs:comment>
        <rdfs:comment xml:lang="en">Lucid: workflow.</rdfs:comment>
        <rdfs:label xml:lang="en">DASH Oversight</rdfs:label>
    </owl:Class>
    


    <!-- http://purl.obolibrary.org/obo/DASH-Onto_0000021 -->

    <owl:Class rdf:about="http://purl.obolibrary.org/obo/DASH-Onto_0000021">
        <obo:IAO_0000115 xml:lang="en">A DASH instruction to a DC, sent by an agreed method, requesting a DC-related project component activity be completed.</obo:IAO_0000115>
        <rdfs:comment xml:lang="en">Lucid: workflow</rdfs:comment>
        <rdfs:label xml:lang="en">Process DASH data custodian instruction</rdfs:label>
    </owl:Class>
    


    <!-- http://purl.obolibrary.org/obo/DASH-Onto_0000026 -->

    <owl:Class rdf:about="http://purl.obolibrary.org/obo/DASH-Onto_0000026">
        <obo:IAO_0000115 xml:lang="en">A process by which a D-SPD is copied to another organisation&apos;s infrastructure or a TEA.</obo:IAO_0000115>
        <rdfs:comment xml:lang="en">DASH: Data placement (DPLACE)</rdfs:comment>
        <rdfs:comment xml:lang="en">Glossary</rdfs:comment>
        <rdfs:label xml:lang="en">Data placement</rdfs:label>
    </owl:Class>
    


    <!-- http://purl.obolibrary.org/obo/DASH-Onto_0000027 -->

    <owl:Class rdf:about="http://purl.obolibrary.org/obo/DASH-Onto_0000027">
        <obo:IAO_0000115 xml:lang="en">A process by which a dataset is generated by applying a function to a set of datasets.</obo:IAO_0000115>
        <rdfs:comment xml:lang="en">Glossary</rdfs:comment>
        <rdfs:label xml:lang="en">Data processing</rdfs:label>
    </owl:Class>
    


    <!-- http://purl.obolibrary.org/obo/DASH-Onto_0000029 -->

    <owl:Class rdf:about="http://purl.obolibrary.org/obo/DASH-Onto_0000029">
        <rdfs:subClassOf rdf:resource="http://purl.obolibrary.org/obo/DASH-Onto_0000027"/>
        <obo:IAO_0000115 xml:lang="en">A data selection by which a project cohort identifier list is generated.</obo:IAO_0000115>
        <rdfs:comment xml:lang="en">DASH: cohort exploration (CEXP)</rdfs:comment>
        <rdfs:comment xml:lang="en">Glossary</rdfs:comment>
        <rdfs:label xml:lang="en">Data custodian Project cohort preparation</rdfs:label>
    </owl:Class>
    


    <!-- http://purl.obolibrary.org/obo/DASH-Onto_0000030 -->

    <owl:Class rdf:about="http://purl.obolibrary.org/obo/DASH-Onto_0000030">
        <rdfs:subClassOf rdf:resource="http://purl.obolibrary.org/obo/DASH-Onto_0000027"/>
        <obo:IAO_0000115 xml:lang="en">A data processing generating a new data asset using a transformation function which has as input a set of datasets.</obo:IAO_0000115>
        <rdfs:comment xml:lang="en">Glossary</rdfs:comment>
        <rdfs:label xml:lang="en">Data transformation</rdfs:label>
    </owl:Class>
    


    <!-- http://purl.obolibrary.org/obo/DASH-Onto_0000031 -->

    <owl:Class rdf:about="http://purl.obolibrary.org/obo/DASH-Onto_0000031">
        <rdfs:subClassOf rdf:resource="http://purl.obolibrary.org/obo/DASH-Onto_0000030"/>
        <obo:IAO_0000115 xml:lang="en">A data processing generating a new data asset using a transformation function which has as input a set of datasets.</obo:IAO_0000115>
        <rdfs:comment xml:lang="en">Glossary</rdfs:comment>
        <rdfs:label xml:lang="en">Data custodian data preparation</rdfs:label>
    </owl:Class>
    


    <!-- http://purl.obolibrary.org/obo/DASH-Onto_0000032 -->

    <owl:Class rdf:about="http://purl.obolibrary.org/obo/DASH-Onto_0000032">
        <rdfs:subClassOf rdf:resource="http://purl.obolibrary.org/obo/DASH-Onto_0000030"/>
        <obo:IAO_0000115 xml:lang="en">A sub-process of data assembly by which privacy enhancing technique functions are applied by a data custodian technical team to the dataset which is the output of the data preparation.</obo:IAO_0000115>
        <rdfs:comment xml:lang="en">Data custodian PET processing</rdfs:comment>
        <rdfs:label xml:lang="en">Data custodian privacy enhancing technique processing</rdfs:label>
    </owl:Class>
    


    <!-- http://purl.obolibrary.org/obo/DASH-Onto_0000035 -->

    <owl:Class rdf:about="http://purl.obolibrary.org/obo/DASH-Onto_0000035">
        <obo:IAO_0000115 xml:lang="en">A project component activity that is TBD.</obo:IAO_0000115>
        <rdfs:comment xml:lang="en">DASH: DASH Project Closure (PCLOSE)</rdfs:comment>
        <rdfs:comment xml:lang="en">Lucid: workflow</rdfs:comment>
        <rdfs:label xml:lang="en">Project debrief</rdfs:label>
    </owl:Class>
    


    <!-- http://purl.obolibrary.org/obo/DASH-Onto_0000037 -->

    <owl:Class rdf:about="http://purl.obolibrary.org/obo/DASH-Onto_0000037">
        <obo:IAO_0000115 xml:lang="en">A DASH instruction to a PRG, sent by an agreed method, requesting a PRG-related project component activity be completed.</obo:IAO_0000115>
        <rdfs:comment xml:lang="en">Lucid: workflow</rdfs:comment>
        <rdfs:label xml:lang="en">Process DASH project research group instruction</rdfs:label>
    </owl:Class>
    


    <!-- http://purl.obolibrary.org/obo/DASH-Onto_0000043 -->

    <owl:Class rdf:about="http://purl.obolibrary.org/obo/DASH-Onto_0000043">
        <obo:IAO_0000115 xml:lang="en">A process by which project research group members include a project analysis data output into an artefact for release to the wider interested community.</obo:IAO_0000115>
        <rdfs:comment xml:lang="en">Glossary</rdfs:comment>
        <rdfs:label xml:lang="en">Project publication drafting</rdfs:label>
    </owl:Class>
    


    <!-- http://purl.obolibrary.org/obo/DASH-Onto_0000045 -->

    <owl:Class rdf:about="http://purl.obolibrary.org/obo/DASH-Onto_0000045">
        <obo:IAO_0000115 xml:lang="en">A review that is TBD.</obo:IAO_0000115>
        <rdfs:comment xml:lang="en">Ont/glossary: proposed</rdfs:comment>
        <rdfs:label xml:lang="en">DC Agreement resource and cost review</rdfs:label>
    </owl:Class>
    


    <!-- http://purl.obolibrary.org/obo/DASH-Onto_0000047 -->

    <owl:Class rdf:about="http://purl.obolibrary.org/obo/DASH-Onto_0000047">
        <obo:IAO_0000115 xml:lang="en">A review performed by a data controller team which evaluates project protocol alignment with its policies and, if applicable, delegated data control agreements</obo:IAO_0000115>
        <rdfs:comment xml:lang="en">DASH: Governance - external (GOVEX)</rdfs:comment>
        <rdfs:comment xml:lang="en">DASH: agreements - external (AGREEEX)</rdfs:comment>
        <rdfs:comment xml:lang="en">Glossary</rdfs:comment>
        <rdfs:label xml:lang="en">Data controller review</rdfs:label>
    </owl:Class>
    


    <!-- http://purl.obolibrary.org/obo/DASH-Onto_0000049 -->

    <owl:Class rdf:about="http://purl.obolibrary.org/obo/DASH-Onto_0000049">
        <obo:IAO_0000115 xml:lang="en">A Data custodian feasibility review that is TBD.</obo:IAO_0000115>
        <rdfs:comment xml:lang="en">Ont: proposed.</rdfs:comment>
        <rdfs:label xml:lang="en">Data Access Request Review</rdfs:label>
    </owl:Class>
    


    <!-- http://purl.obolibrary.org/obo/DASH-Onto_0000050 -->

    <owl:Class rdf:about="http://purl.obolibrary.org/obo/DASH-Onto_0000050">
        <obo:IAO_0000115 xml:lang="en">A review performed by a data custodian team in collaboration with a project research group which assesses whether the [cohort] data item requirements defined by a project protocol can be fullfilled by a data custodian.</obo:IAO_0000115>
        <rdfs:comment xml:lang="en">Glossary</rdfs:comment>
        <rdfs:label xml:lang="en">Data availability cohort review</rdfs:label>
    </owl:Class>
    


    <!-- http://purl.obolibrary.org/obo/DASH-Onto_0000051 -->

    <owl:Class rdf:about="http://purl.obolibrary.org/obo/DASH-Onto_0000051">
        <obo:IAO_0000115 xml:lang="en">A review performed by a data custodian team in collaboration with a project research group which assesses whether the [extract] data item requirements defined by a project protocol can be fullfilled by a data custodian.</obo:IAO_0000115>
        <rdfs:comment xml:lang="en">Glossary</rdfs:comment>
        <rdfs:label xml:lang="en">Data availability extract review</rdfs:label>
    </owl:Class>
    


    <!-- http://purl.obolibrary.org/obo/DASH-Onto_0000052 -->

    <owl:Class rdf:about="http://purl.obolibrary.org/obo/DASH-Onto_0000052">
        <obo:IAO_0000115 xml:lang="en">An eligibility review performed by a data custodian team which uses custodian-defined governance criteria to establish the right of the project research group to have a project protocol evaluated by the DCG team.</obo:IAO_0000115>
        <rdfs:comment xml:lang="en">DASH: Eligibility Review (ELREV)</rdfs:comment>
        <rdfs:comment xml:lang="en">Glossary</rdfs:comment>
        <rdfs:label xml:lang="en">Data eligibility review</rdfs:label>
    </owl:Class>
    


    <!-- http://purl.obolibrary.org/obo/DASH-Onto_0000053 -->

    <owl:Class rdf:about="http://purl.obolibrary.org/obo/DASH-Onto_0000053">
        <obo:IAO_0000115 xml:lang="en">A review performed by a data custodian team which determines costs and resources required to provide access to data items, and other requested services options (if applicable).</obo:IAO_0000115>
        <rdfs:comment xml:lang="en">DASH: Cost and resource review (COSTREV)</rdfs:comment>
        <rdfs:comment xml:lang="en">Glossary</rdfs:comment>
        <rdfs:label xml:lang="en">Data estimated resource cost review</rdfs:label>
    </owl:Class>
    


    <!-- http://purl.obolibrary.org/obo/DASH-Onto_0000055 -->

    <owl:Class rdf:about="http://purl.obolibrary.org/obo/DASH-Onto_0000055">
        <obo:IAO_0000115 xml:lang="en">A application element review which ensures that appropriate documentation arising from an ethics committee assessment was submitted as part of an application process.</obo:IAO_0000115>
        <rdfs:comment xml:lang="en">Glossary</rdfs:comment>
        <rdfs:label xml:lang="en">Ethics assessment review</rdfs:label>
    </owl:Class>
    


    <!-- http://purl.obolibrary.org/obo/DASH-Onto_0000056 -->

    <owl:Class rdf:about="http://purl.obolibrary.org/obo/DASH-Onto_0000056">
        <obo:IAO_0000115 xml:lang="en">A application element review which ensures that an appropriate documentation from some funding source was submitted as part of an application process.</obo:IAO_0000115>
        <rdfs:comment xml:lang="en">Glossary</rdfs:comment>
        <rdfs:label xml:lang="en">Funding review</rdfs:label>
    </owl:Class>
    


    <!-- http://purl.obolibrary.org/obo/DASH-Onto_0000057 -->

    <owl:Class rdf:about="http://purl.obolibrary.org/obo/DASH-Onto_0000057">
        <obo:IAO_0000115 xml:lang="en">A Data custodian governance review that is TBD.</obo:IAO_0000115>
        <rdfs:comment xml:lang="en">Glossary</rdfs:comment>
        <rdfs:label xml:lang="en">Non-disclosure agreement review</rdfs:label>
    </owl:Class>
    


    <!-- http://purl.obolibrary.org/obo/DASH-Onto_0000058 -->

    <owl:Class rdf:about="http://purl.obolibrary.org/obo/DASH-Onto_0000058">
        <obo:IAO_0000115 xml:lang="en">An review with the goal of ensuring that privacy and patient-practitioner confidentiality are not compromised during processes directed by the project protocol.</obo:IAO_0000115>
        <rdfs:comment xml:lang="en">Glossary</rdfs:comment>
        <rdfs:label xml:lang="en">Privacy, Confidentiality and Security Review</rdfs:label>
    </owl:Class>
    


    <!-- http://purl.obolibrary.org/obo/DASH-Onto_0000059 -->

    <owl:Class rdf:about="http://purl.obolibrary.org/obo/DASH-Onto_0000059">
        <obo:IAO_0000115 xml:lang="en">A Data custodian governance review that is TBD.</obo:IAO_0000115>
        <rdfs:comment xml:lang="en">Glossary</rdfs:comment>
        <rdfs:label xml:lang="en">Privacy Enhancing Technique Review</rdfs:label>
    </owl:Class>
    


    <!-- http://purl.obolibrary.org/obo/DASH-Onto_0000060 -->

    <owl:Class rdf:about="http://purl.obolibrary.org/obo/DASH-Onto_0000060">
        <obo:IAO_0000115 xml:lang="en">A review conducted by a data controller team to evaluate whether a project analysis data output can be transferred to a different data custodian as requested by a PRG.</obo:IAO_0000115>
        <rdfs:comment xml:lang="en">Glossary</rdfs:comment>
        <rdfs:label xml:lang="en">Project analysis data output review</rdfs:label>
    </owl:Class>
    


    <!-- http://purl.obolibrary.org/obo/DASH-Onto_0000061 -->

    <owl:Class rdf:about="http://purl.obolibrary.org/obo/DASH-Onto_0000061">
        <obo:IAO_0000115 xml:lang="en">An application element review which ensures that appropriate documentation arising from a Scientific Peer review assessment was submitted as part of an application process.</obo:IAO_0000115>
        <rdfs:comment xml:lang="en">Glossary</rdfs:comment>
        <rdfs:label xml:lang="en">Scientific assessment review</rdfs:label>
    </owl:Class>
    


    <!-- http://purl.obolibrary.org/obo/DASH-Onto_0000062 -->

    <owl:Class rdf:about="http://purl.obolibrary.org/obo/DASH-Onto_0000062">
        <obo:IAO_0000115 xml:lang="en">A review conducted by a organisation team to evaluate whether a project publication candidate can be made available outside the project research group.</obo:IAO_0000115>
        <rdfs:comment xml:lang="en">Glossary</rdfs:comment>
        <rdfs:label xml:lang="en">Project publication review</rdfs:label>
    </owl:Class>
    


    <!-- http://purl.obolibrary.org/obo/DASH-Onto_0000063 -->

    <owl:Class rdf:about="http://purl.obolibrary.org/obo/DASH-Onto_0000063">
        <obo:IAO_0000115 xml:lang="en">A TEA feasibility review that is TBD.</obo:IAO_0000115>
        <rdfs:comment xml:lang="en">Ont/glossary: proposed.</rdfs:comment>
        <rdfs:label xml:lang="en">TEA Agreement resource and cost review</rdfs:label>
    </owl:Class>
    


    <!-- http://purl.obolibrary.org/obo/DASH-Onto_0000066 -->

    <owl:Class rdf:about="http://purl.obolibrary.org/obo/DASH-Onto_0000066">
        <obo:IAO_0000115 xml:lang="en">A TEA feasibility review that is TBD.</obo:IAO_0000115>
        <rdfs:comment xml:lang="en">Ont/glossary: proposed.</rdfs:comment>
        <rdfs:label xml:lang="en">TEA eligibility review</rdfs:label>
    </owl:Class>
    


    <!-- http://purl.obolibrary.org/obo/DASH-Onto_0000067 -->

    <owl:Class rdf:about="http://purl.obolibrary.org/obo/DASH-Onto_0000067">
        <obo:IAO_0000115 xml:lang="en">A TEA feasibility review that is TBD.</obo:IAO_0000115>
        <rdfs:comment xml:lang="en">Ont/glossary: proposed.</rdfs:comment>
        <rdfs:label xml:lang="en">TEA estimated resource and cost review</rdfs:label>
    </owl:Class>
    


    <!-- http://purl.obolibrary.org/obo/DASH-Onto_0000068 -->

    <owl:Class rdf:about="http://purl.obolibrary.org/obo/DASH-Onto_0000068">
        <obo:IAO_0000115 xml:lang="en">A TEA feasibility review that is TBD.</obo:IAO_0000115>
        <rdfs:comment xml:lang="en">DASH: Requested services review (SREV)</rdfs:comment>
        <rdfs:comment xml:lang="en">Ont/glossary: proposed.</rdfs:comment>
        <rdfs:label xml:lang="en">TEA support review</rdfs:label>
    </owl:Class>
    


    <!-- http://purl.obolibrary.org/obo/DASH-Onto_0000080 -->

    <owl:Class rdf:about="http://purl.obolibrary.org/obo/DASH-Onto_0000080">
        <obo:IAO_0000115 xml:lang="en">TBD.</obo:IAO_0000115>
        <rdfs:label xml:lang="en">Wait for signal</rdfs:label>
    </owl:Class>
    


    <!-- http://purl.obolibrary.org/obo/DASH-Onto_0000081 -->

    <owl:Class rdf:about="http://purl.obolibrary.org/obo/DASH-Onto_0000081">
        <obo:IAO_0000115 xml:lang="en">TBD.</obo:IAO_0000115>
        <rdfs:label xml:lang="en">Send signal</rdfs:label>
    </owl:Class>
    


    <!-- http://purl.obolibrary.org/obo/DASH-Onto_0000082 -->

    <owl:Class rdf:about="http://purl.obolibrary.org/obo/DASH-Onto_0000082">
        <obo:IAO_0000115 xml:lang="en">A project research group activity by which one or more project research group members demonstrate knowledge of the requirements that a data custodian places on the use and handling of D-SPD provided to ensure continued good governance of that D-SPD and associated project analysis and publication.</obo:IAO_0000115>
        <rdfs:label xml:lang="en">Project research group orientation validation</rdfs:label>
    </owl:Class>
    


    <!-- http://purl.obolibrary.org/obo/DASH-Onto_0000083 -->

    <owl:Class rdf:about="http://purl.obolibrary.org/obo/DASH-Onto_0000083">
        <obo:IAO_0000115 xml:lang="en">A DASH instruction to a DC, sent by an agreed method, requesting a TEA-related project component activity be completed.</obo:IAO_0000115>
        <rdfs:label xml:lang="en">Process DASH trusted environment for analysis instruction</rdfs:label>
    </owl:Class>
    


    <!-- http://purl.obolibrary.org/obo/DASH-Onto_0000084 -->

    <owl:Class rdf:about="http://purl.obolibrary.org/obo/DASH-Onto_0000084">
        <obo:IAO_0000115 xml:lang="en">A project component activity that permits DASH to restart DC-specific TEA activities and communicate this fact to the DC, the latter taking appropriate actions in response.</obo:IAO_0000115>
        <rdfs:label xml:lang="en">DASH TEA Monitor process</rdfs:label>
    </owl:Class>
    


    <!-- http://purl.obolibrary.org/obo/DASH-Onto_0000085 -->

    <owl:Class rdf:about="http://purl.obolibrary.org/obo/DASH-Onto_0000085">
        <obo:IAO_0000115 xml:lang="en">A project component activity that permits DASH to restart DC-specific DC activities and communicate this fact to the DC, the latter taking appropriate actions in response.</obo:IAO_0000115>
        <rdfs:label xml:lang="en">DASH DC Monitor process</rdfs:label>
    </owl:Class>
</rdf:RDF>



<!-- Generated by the OWL API (version 4.5.26) https://github.com/owlcs/owlapi -->

